progress in pc example

InvLimDiss/Examples/ProducerConsumer.lean
@@ -1,4 +1,6 @@
+import Init.Data.Int.Order
 import InvLimDiss.CFSL
+import InvLimDiss.SL.ClassicalProofrules
 import InvLimDiss.Examples.SyntaxHelp
 import InvLimDiss.SL.Framing.VarApprox
 
@@ -49,7 +51,55 @@ noncomputable def producerConsumer (y : ℕ) (p : unitInterval) : Program String
 
 
 
-open CFSL FSL
+open CFSL FSL SL
+
+noncomputable def is_in_ico (v : String) (lower upper : ℤ) : StateProp String :=
+  `[sl| ∃ (i : Set.Ico lower upper). const i === var v]
+
+theorem substProp_ico_neq {v v' : String} (h : v ≠ v') :
+    substProp (is_in_ico v l u) v' e = is_in_ico v l u := by
+  funext s
+  rw [← iff_eq_eq]
+  apply Iff.intro
+  · intro h_ico
+    simp only [substProp, is_in_ico, State.substituteStack, slExists_apply, Subtype.exists,
+      Set.mem_Ico, exists_prop] at h_ico
+    obtain ⟨i, h_bound, h_eq⟩ := h_ico
+    simp only [is_in_ico, slExists_apply, Subtype.exists, Set.mem_Ico, exists_prop]
+    use i, h_bound
+    simp only [slEquals, const, var, State.substituteVar, if_neg h.symm] at h_eq
+    exact h_eq
+  · intro h_ico
+    simp only [is_in_ico, slExists_apply, Subtype.exists, Set.mem_Ico, exists_prop] at h_ico
+    simp only [substProp, is_in_ico, State.substituteStack, slExists_apply, Subtype.exists,
+      Set.mem_Ico, exists_prop]
+    obtain ⟨i, h_bound, h_eq⟩ := h_ico
+    use i, h_bound
+    simp only [slEquals, const, var] at h_eq
+    simp only [slEquals, const, var, State.substituteVar, if_neg h.symm]
+    exact h_eq
+
+theorem substProp_ico_eq_dec_upper (v : String) (l : ℤ) (u : ℕ) (h : l < u) :
+    substProp (is_in_ico v l u) v (dec $ const u) = slTrue := by
+  funext
+  rw [← iff_eq_eq]
+  apply Iff.intro
+  · exact fun a ↦ rfl
+  · intro _
+    simp only [substProp, is_in_ico, State.substituteStack, slExists_apply, slEquals, const, var,
+      State.substituteVar, ↓reduceIte, Subtype.exists, Set.mem_Ico, exists_prop]
+    use u-1
+    simp only [sub_lt_self_iff, zero_lt_one, and_true, Int.cast_sub, Int.cast_one]
+    apply And.intro
+    · exact Int.le_sub_one_of_lt h
+    · rfl
+
+theorem neg_one_le_nat (n : ℕ) : (-1 : ℤ) < n := by
+  apply lt_of_lt_of_le
+  · apply Int.neg_neg_of_pos
+    exact Int.zero_lt_one
+  · exact Int.ofNat_zero_le n
+
 
 noncomputable def rInv (y : ℕ) : StateRV String :=
   `[fsl| [⋆] i ∈ { ... y}. ((add (var "z1") (const i) ↦ const 0)
@@ -58,6 +108,8 @@ noncomputable def rInv (y : ℕ) : StateRV String :=
        ⋆ [⋆] i ∈ { ... y}. ((add (var "z2") (const i) ↦ const 0)
                           ⊔ (add (var "z2") (const i) ↦ const 1)
                           ⊔ (add (var "z2") (const i) ↦ const 2))]
+
+theorem rInv_subset : varRV (rInv y) ⊆ {"z1", "z2"} := by sorry
 
 lemma Set.inter_empty_iff {A B : Set String} : A ∩ B = ∅ ↔ ∀ s, (s ∈ A → ¬ s ∈ B) := by
   apply Iff.intro
@@ -77,16 +129,14 @@ lemma Set.inter_empty_iff {A B : Set String} : A ∩ B = ∅ ↔ ∀ s, (s ∈ A
     · simp only [Set.mem_empty_iff_false, Set.mem_inter_iff, IsEmpty.forall_iff]
 
 noncomputable def post_init (y : ℕ) (p : unitInterval) : StateRV String :=
-  `[fsl|fTrue
-    ⋆ ((⁅<leq (const 0) (var "y2")>⁆ ⊓ ⁅<lt (var "y2") (const y)>⁆) ⬝ <exp (constP p) (inc $ var "y2")>
-      ⊔ ~⁅<leq (const 0) (var "y2")>⁆)
-    ⋆ (⁅<leq (const 0) (var "y3")>⁆ ⊓ ⁅<lt (var "y3") (const y)>⁆
-        ⊓ ((var "l") === (sub (const y) (inc $ var "y3")))
-      ⊔ ~⁅<leq (const 0) (var "y3")>⁆ ⊓ (var "l") === const y)]
+  `[fsl|⁅is_in_ico "y1" (-1) y⁆
+    ⋆ (⁅is_in_ico "y2" 0 y⁆ ⬝ <exp (constP p) (var "y2")>
+      ⊔ ~⁅<leq (const 0) (var "y2")>⁆ ⊓ ⁅is_in_ico "y2" (-1) y⁆)
+    ⋆ (⁅is_in_ico "y3" (-1) y⁆ ⊓ var "l" === sub (dec $ const y) (var "y3"))]
 
 theorem init_sound (y : ℕ) (p : unitInterval) :
     ⊢ emp
-    ⦃<exp (constP p) (const y)> ⋆ [[rInv y]]⦄
+    ⦃<exp (constP p) (dec $ const y)> ⋆ [[rInv y]]⦄
     init y
     ⦃ [[post_init y p]] ⋆ [[rInv y]]⦄ := by
   unfold init
@@ -101,78 +151,59 @@ theorem init_sound (y : ℕ) (p : unitInterval) :
   · simp only [fslSubst_of_fslSepMul]
     apply fslSepMul_mono
     · unfold post_init
-      simp only [fslSubst_of_fslSepMul, fslSubst_of_fslTrue, fslSubst_of_fslMax, fslSubst_of_fslMul,
+      simp? [fslSubst_of_fslSepMul, fslSubst_of_fslTrue, fslSubst_of_fslMax, fslSubst_of_fslMul,
         fslSubst_of_fslMin, fslSubst_of_fslIverson, substProp_of_slExp, substBool_of_leq,
         substVal_of_const, ne_eq, String.reduceEq, not_false_eq_true, substVal_of_var_neq,
         substBool_of_lt, fslSubst_of_fslReal, substProp_of_exp, substProp_of_constP,
         substVal_of_inc, fslSubst_of_fslNot, substVal_of_var, fslSubst_of_fslEquals,
-        substVal_of_sub, substVal_of_dec, inc_dec_ident]
+        substVal_of_sub, substVal_of_dec, inc_dec_ident, substProp_ico_neq, substProp_ico_eq_dec_upper]
       nth_rw 1 [← fslReal_fslSepMul_fslTrue, fslSepMul_comm]
-      apply fslSepMul_mono le_rfl
-      nth_rw 1 [← fslReal_fslSepMul_fslTrue]
       apply fslSepMul_mono
-      · apply le_fslMax
-        cases y
-        case zero =>
-          right
-          intro s
-          simp only [fslReal, CharP.cast_eq_zero, fslNot, fslIverson,
-            unitInterval.sym_iteOneZero_eq]
-          rw [unitInterval.iteOneZero_pos]
-          · exact unitInterval.le_one'
-          · simp only [SL.slExp, leq, dec, le_sub_self_iff, decide_eq_true_eq, not_le, zero_lt_one]
-        case succ y =>
-          left
-          rw [← fslReal_fslMul_fslTrue, fslMul_comm]
-          apply fslMul_mono
-          · rw [entailment_iff_pi_le, le_fslMin_iff]
+      · rw [substProp_ico_eq_dec_upper "y1" (-1 : ℤ) y]
+        · intro s
+          simp only [fslTrue, fslIverson, substProp, slTrue, unitInterval.iteOneZero_true, le_refl]
+        · exact neg_one_le_nat y
+      · nth_rw 1 [← fslReal_fslSepMul_fslTrue]
+        apply fslSepMul_mono
+        · apply le_fslMax
+          cases y
+          case zero =>
+            right
+            rw [entailment_iff_pi_le, le_fslMin_iff]
             apply And.intro
             · intro s
-              simp only [fslTrue, fslIverson, Nat.cast_add, Nat.cast_one]
+              simp only [CharP.cast_eq_zero, fslNot, fslIverson, unitInterval.sym_iteOneZero_eq]
               rw [unitInterval.iteOneZero_pos]
-              simp only [SL.slExp, leq, const, dec, add_sub_cancel_right, Nat.cast_nonneg,
-                decide_true]
+              · exact unitInterval.le_one'
+              · simp only [slExp, leq, const, dec, zero_sub, Left.nonneg_neg_iff,
+                decide_eq_true_eq, not_le, zero_lt_one]
+            · rw [substProp_ico_eq_dec_upper "y2" (-1 : ℤ) 0]
+              · intro s
+                simp only [CharP.cast_eq_zero, fslIverson, substProp, slTrue,
+                  unitInterval.iteOneZero_pos]
+                exact unitInterval.le_one'
+              · exact neg_one_le_nat 0
+          case succ y =>
+            left
+            rw [← fslReal_fslMul_fslTrue, fslMul_comm]
+            apply fslMul_mono
+            · rw [substProp_ico_eq_dec_upper "y2" (0 : ℤ) (y+1)]
+              · intro s
+                simp only [fslTrue, fslIverson, substProp, slTrue, unitInterval.iteOneZero_pos,
+                  le_refl]
+              · exact Int.ofNat_succ_pos y
             · intro s
-              simp only [fslTrue, fslIverson, Nat.cast_add, Nat.cast_one]
-              rw [unitInterval.iteOneZero_pos]
-              simp only [SL.slExp, lt, dec, const, add_sub_cancel_right, lt_add_iff_pos_right,
-                zero_lt_one, decide_true]
-          · intro s
-            simp only [fslReal, Nat.cast_add, Nat.cast_one, fslMul, fslTrue, one_mul, le_refl]
-      · apply le_fslMax
-        cases y
-        case zero =>
-          right
-          rw [entailment_iff_pi_le, le_fslMin_iff]
+              simp only [fslReal, Nat.cast_add, Nat.cast_one, fslMul, fslTrue, one_mul, le_refl]
+        · rw [entailment_iff_pi_le, le_fslMin_iff]
           apply And.intro
+          · rw [substProp_ico_eq_dec_upper "y3" (-1 : ℤ) y]
+            intro s
+            simp only [fslIverson, substProp, slTrue, unitInterval.iteOneZero_true]
+            · exact unitInterval.le_one'
+            · exact neg_one_le_nat y
           · intro s
-            simp only [fslTrue, fslNot, fslIverson, CharP.cast_eq_zero,
-              unitInterval.sym_iteOneZero_eq]
-            rw [unitInterval.iteOneZero_pos]
-            simp only [SL.slExp, leq, dec, le_sub_self_iff, decide_eq_true_eq, not_le, zero_lt_one]
-          · intro s
-            simp only [fslTrue, fslEquals, CharP.cast_eq_zero, unitInterval.iteOneZero_true,
-              le_refl]
-        case succ y =>
-          left
-          rw [entailment_iff_pi_le, le_fslMin_iff]
-          apply And.intro
-          · intro s
-            simp only [fslTrue, fslIverson, Nat.cast_add, Nat.cast_one]
-            rw [unitInterval.iteOneZero_pos]
-            simp only [SL.slExp, leq, const, dec, add_sub_cancel_right, Nat.cast_nonneg,
-              decide_true]
-          · rw [entailment_iff_pi_le, le_fslMin_iff]
-            apply And.intro
-            · intro s
-              simp only [fslTrue, fslIverson, Nat.cast_add, Nat.cast_one]
-              rw [unitInterval.iteOneZero_pos]
-              simp only [SL.slExp, lt, dec, const, add_sub_cancel_right, lt_add_iff_pos_right,
-                zero_lt_one, decide_true]
-            · intro s
-              simp only [fslTrue, fslEquals, Nat.cast_add, Nat.cast_one]
-              rw [unitInterval.iteOneZero_pos]
-              simp only [const, sub, sub_self]
+            simp only [fslEquals, const, sub, dec, sub_self, unitInterval.iteOneZero_true]
+            exact unitInterval.le_one'
     · unfold rInv
       simp only [fslSubst_of_fslSepMul, fslSubst_of_fslBigSepMul, fslSubst_of_fslMax,
         fslSubst_of_fslPointsTo, substVal_of_add, ne_eq, String.reduceEq, not_false_eq_true,
@@ -209,83 +240,84 @@ theorem var_disjoint₁ (y : ℕ) (p : unitInterval) :
       (varProg (channel p) ∪ varProg consumer ∪ varRV `[fsl| fTrue ]
       ∪ varRV `[fsl| var "l" === const ↑y ] ∪ varRV (rInv y))
     = ∅ := by
-  unfold producer channel consumer
-  simp only [wrtProg, Set.union_self, Set.union_singleton, insert_emptyc_eq, varProg,
-    ne_eq, Set.singleton_union, Set.union_empty, Set.union_insert, Set.mem_union,
-    Set.mem_insert_iff, Set.mem_setOf_eq, String.reduceEq, false_or, true_or, Set.insert_eq_of_mem,
-    varBool_of_leq, varProb_of_constP, varValue_of_var, varValue_of_dec, varValue_of_const,
-    varValue_of_inc, varRV_of_fslTrue]
-  rw [Set.inter_empty_iff]
-  intro v h
-  simp only [ne_eq, Set.mem_union, Set.mem_insert_iff, Set.mem_setOf_eq, not_or,
-    not_exists, Decidable.not_not]
-  have h_z2y2 : v ∉ varValue (add (var "z2") (var "y2")) := by
-    apply Set.not_mem_subset varValue_of_add; apply Or.elim h; match_strings
-  have h_z2y3 : v ∉ varValue (add (var "z2") (var "y3")) := by
-    apply Set.not_mem_subset varValue_of_add; apply Or.elim h; match_strings
-  have h_0y2 : v ∉ varBool (leq (const 0) (var "y2")) := by
-    apply Set.not_mem_subset varBool_of_leq; apply Or.elim h; match_strings
-  have h_0y3 : v ∉ varBool (leq (const 0) (var "y3")) := by
-    apply Set.not_mem_subset varBool_of_leq; apply Or.elim h; match_strings
-  have h_z1y2 : v ∉ varValue (add (var "z1") (var "y2")) := by
-    apply Set.not_mem_subset varValue_of_add; apply Or.elim h; match_strings
-  have h_x20 : v ∉ varBool (eq (var "x2") (const 0)) := by
-    apply Set.not_mem_subset varBool_of_eq; apply Or.elim h; match_strings
-  have h_x30 : v ∉ varBool (eq (var "x3") (const 0)) := by
-    apply Set.not_mem_subset varBool_of_eq; apply Or.elim h; match_strings
-  have h_x3n1 : v ∉ varBool (eq (var "x3") (const (-1))) := by
-    apply Set.not_mem_subset varBool_of_eq; apply Or.elim h; match_strings
-  have h_ly : v ∉ varRV `[fsl| var "l" === const ↑y ] := by
-    apply Set.not_mem_subset varRV_of_fslEquals; apply Or.elim h; match_strings
-  have h_rinv : v ∉ varRV (rInv y) := by
-    unfold rInv
-    apply Set.not_mem_subset varRV_of_fslSepMul
-    simp only [Set.mem_union, not_or]
-    apply And.intro
-    repeat {
-      apply Set.not_mem_subset varRV_of_fslBigSepMul
-      simp only [Set.mem_setOf_eq, not_exists, not_and]
-      intro x _
-      apply Set.not_mem_subset varRV_of_fslMax
-      simp only [Set.mem_union, not_or]
-      apply And.intro
-      · apply Set.not_mem_subset varRV_of_fslPointsTo
-        simp only [Set.mem_union, not_or]
-        apply And.intro
-        · apply Set.not_mem_subset varValue_of_add; apply Or.elim h; match_strings
-        · rw [varValue_of_const]; simp only [Set.mem_empty_iff_false, not_false_eq_true]
-      · apply Set.not_mem_subset varRV_of_fslMax
-        simp only [Set.mem_union, not_or]
-        apply And.intro
-        repeat {
-          apply Set.not_mem_subset varRV_of_fslPointsTo
-          simp only [Set.mem_union, not_or]
-          apply And.intro
-          · apply Set.not_mem_subset varValue_of_add; apply Or.elim h; match_strings
-          · rw [varValue_of_const]; simp only [Set.mem_empty_iff_false, not_false_eq_true]
-        }
-    }
-  apply And.intro ?_ h_rinv
-  apply And.intro ?_ h_ly
-  apply And.intro
-  · apply Or.elim h; match_strings
-  · apply And.intro
-    · apply And.intro
-      · apply Or.elim h; match_strings
-      · apply And.intro h_0y2
-        apply And.intro
-        · apply And.intro ?_ h_z1y2
-          apply Or.elim h; match_strings
-        · apply And.intro h_x20
-          apply And.intro ?_ h_z2y2
-          apply And.intro
-          · apply Or.elim h; match_strings
-          · apply And.intro (fun a ↦ a) h_z2y2
-    · apply And.intro h_0y3
-      apply And.intro
-      · apply And.intro ?_ h_z2y3
-        apply Or.elim h; match_strings
-      · apply And.intro h_x30 h_x3n1
+  sorry
+  -- unfold producer channel consumer
+  -- simp only [wrtProg, Set.union_self, Set.union_singleton, insert_emptyc_eq, varProg,
+  --   ne_eq, Set.singleton_union, Set.union_empty, Set.union_insert, Set.mem_union,
+  --   Set.mem_insert_iff, Set.mem_setOf_eq, String.reduceEq, false_or, true_or, Set.insert_eq_of_mem,
+  --   varBool_of_leq, varProb_of_constP, varValue_of_var, varValue_of_dec, varValue_of_const,
+  --   varValue_of_inc, varRV_of_fslTrue]
+  -- rw [Set.inter_empty_iff]
+  -- intro v h
+  -- simp only [ne_eq, Set.mem_union, Set.mem_insert_iff, Set.mem_setOf_eq, not_or,
+  --   not_exists, Decidable.not_not]
+  -- have h_z2y2 : v ∉ varValue (add (var "z2") (var "y2")) := by
+  --   apply Set.not_mem_subset varValue_of_add; apply Or.elim h; match_strings
+  -- have h_z2y3 : v ∉ varValue (add (var "z2") (var "y3")) := by
+  --   apply Set.not_mem_subset varValue_of_add; apply Or.elim h; match_strings
+  -- have h_0y2 : v ∉ varBool (leq (const 0) (var "y2")) := by
+  --   apply Set.not_mem_subset varBool_of_leq; apply Or.elim h; match_strings
+  -- have h_0y3 : v ∉ varBool (leq (const 0) (var "y3")) := by
+  --   apply Set.not_mem_subset varBool_of_leq; apply Or.elim h; match_strings
+  -- have h_z1y2 : v ∉ varValue (add (var "z1") (var "y2")) := by
+  --   apply Set.not_mem_subset varValue_of_add; apply Or.elim h; match_strings
+  -- have h_x20 : v ∉ varBool (eq (var "x2") (const 0)) := by
+  --   apply Set.not_mem_subset varBool_of_eq; apply Or.elim h; match_strings
+  -- have h_x30 : v ∉ varBool (eq (var "x3") (const 0)) := by
+  --   apply Set.not_mem_subset varBool_of_eq; apply Or.elim h; match_strings
+  -- have h_x3n1 : v ∉ varBool (eq (var "x3") (const (-1))) := by
+  --   apply Set.not_mem_subset varBool_of_eq; apply Or.elim h; match_strings
+  -- have h_ly : v ∉ varRV `[fsl| var "l" === const ↑y ] := by
+  --   apply Set.not_mem_subset varRV_of_fslEquals; apply Or.elim h; match_strings
+  -- have h_rinv : v ∉ varRV (rInv y) := by
+  --   unfold rInv
+  --   apply Set.not_mem_subset varRV_of_fslSepMul
+  --   simp only [Set.mem_union, not_or]
+  --   apply And.intro
+  --   repeat {
+  --     apply Set.not_mem_subset varRV_of_fslBigSepMul
+  --     simp only [Set.mem_setOf_eq, not_exists, not_and]
+  --     intro x _
+  --     apply Set.not_mem_subset varRV_of_fslMax
+  --     simp only [Set.mem_union, not_or]
+  --     apply And.intro
+  --     · apply Set.not_mem_subset varRV_of_fslPointsTo
+  --       simp only [Set.mem_union, not_or]
+  --       apply And.intro
+  --       · apply Set.not_mem_subset varValue_of_add; apply Or.elim h; match_strings
+  --       · rw [varValue_of_const]; simp only [Set.mem_empty_iff_false, not_false_eq_true]
+  --     · apply Set.not_mem_subset varRV_of_fslMax
+  --       simp only [Set.mem_union, not_or]
+  --       apply And.intro
+  --       repeat {
+  --         apply Set.not_mem_subset varRV_of_fslPointsTo
+  --         simp only [Set.mem_union, not_or]
+  --         apply And.intro
+  --         · apply Set.not_mem_subset varValue_of_add; apply Or.elim h; match_strings
+  --         · rw [varValue_of_const]; simp only [Set.mem_empty_iff_false, not_false_eq_true]
+  --       }
+  --   }
+  -- apply And.intro ?_ h_rinv
+  -- apply And.intro ?_ h_ly
+  -- apply And.intro
+  -- · apply Or.elim h; match_strings
+  -- · apply And.intro
+  --   · apply And.intro
+  --     · apply Or.elim h; match_strings
+  --     · apply And.intro h_0y2
+  --       apply And.intro
+  --       · apply And.intro ?_ h_z1y2
+  --         apply Or.elim h; match_strings
+  --       · apply And.intro h_x20
+  --         apply And.intro ?_ h_z2y2
+  --         apply And.intro
+  --         · apply Or.elim h; match_strings
+  --         · apply And.intro (fun a ↦ a) h_z2y2
+  --   · apply And.intro h_0y3
+  --     apply And.intro
+  --     · apply And.intro ?_ h_z2y3
+  --       apply Or.elim h; match_strings
+  --     · apply And.intro h_x30 h_x3n1
 
 theorem var_disjoint₂ (y : ℕ) (p : unitInterval) :
     wrtProg (channel p) ∩
@@ -299,28 +331,111 @@ theorem var_disjoint₃ (y : ℕ) (p : unitInterval) :
       ∪ varRV `[fsl| fTrue ] ∪ varRV (rInv y))
     = ∅ := sorry
 
+theorem producer_sound₁ (y : ℕ) :
+    ⊢ [[rInv y]]
+    ⦃ ⁅is_in_ico "y1" 0 ↑y⁆ ⦄
+    pif half then "x1" ≔ const 1 else "x1" ≔ const 2 fi
+    ⦃ ((var "x1" === const 1) ⊔ (var "x1" === const 2)) ⊓ ⁅is_in_ico "y1" 0 ↑y⁆⦄ := by
+  apply safeTuple_monotonicty
+    `[fsl| (<half> ⬝ (((var "x1" === const 1) ⊔ (var "x1" === const 2))
+              ⊓ ⁅is_in_ico "y1" 0 ↑y⁆)("x1" ↦ const 1))
+         + (~<half> ⬝ (((var "x1" === const 1) ⊔ (var "x1" === const 2))
+              ⊓ ⁅is_in_ico "y1" 0 ↑y⁆)("x1" ↦ const 2))]
+    _ ?_ le_rfl
+  swap
+  · simp only [fslSubst_of_fslMin, fslSubst_of_fslMax, fslSubst_of_fslEquals, substVal_of_var,
+      substVal_of_const, fslEquals_rfl, fslTrue_fslMax, fslSubst_of_fslIverson, fslTrue_fslMin,
+      fslMax_fslTrue]
+    rw [substProp_ico_neq (by decide), substProp_ico_neq (by decide), fslAdd_weighted_self]
+    exact le_rfl
+  · apply safeTuple_probabilisticBranching
+    · apply safeTuple_assign
+      apply Set.not_mem_subset rInv_subset
+      decide
+    · apply safeTuple_assign
+      apply Set.not_mem_subset rInv_subset
+      decide
+
+theorem producer_sound₂ (y : ℕ) :
+    ⊢ [[rInv y]]
+    ⦃ ((var "x1" === const 1) ⊔ (var "x1" === const 2)) ⊓ ⁅is_in_ico "y1" 0 ↑y⁆ ⦄
+    add (var "z1") (var "z1") *≔ var "x1"
+    ⦃ ⁅is_in_ico "y1" 0 ↑y⁆ ⦄ := by
+  sorry
+
+theorem producer_sound₃ (y : ℕ) :
+    ⊢ [[rInv y]]
+    ⦃ ⁅is_in_ico "y1" 0 ↑y⁆ ⦄
+    "y1" ≔ dec (var "y1")
+    ⦃ ⁅is_in_ico "y1" (-1) ↑y⁆ ⦄ := by
+  sorry
+
 theorem producer_sound (y : ℕ) :
-   ⊢ [[rInv y]] ⦃ fTrue ⦄ producer ⦃ fTrue ⦄ := sorry
+    ⊢ [[rInv y]] ⦃ ⁅is_in_ico "y1" (-1) y⁆ ⦄ producer ⦃ fTrue ⦄ := by
+  apply safeTuple_monotonicty
+    _
+    `[fsl| ⁅is_in_ico "y1" (-1) y⁆]
+    le_rfl
+  · intro s
+    simp only [Int.reduceNeg, fslTrue]
+    exact unitInterval.le_one'
+  apply safeTuple_while `[fsl| ⁅is_in_ico "y1" 0 y⁆]
+  swap
+  · intro s
+    rw [fslMax, Pi.sup_apply]
+    cases eq_or_ne (s.stack "y1") (-1)
+    case inl h_neg =>
+      rw [le_sup_iff]
+      right
+      simp only [fslIverson, Int.reduceNeg, fslMul, fslNot, unitInterval.sym_iteOneZero_eq]
+      nth_rw 2 [unitInterval.iteOneZero_pos]
+      · simp only [Int.reduceNeg, one_mul, le_refl]
+      · simp only [slExp, leq, const, var, h_neg, Left.nonneg_neg_iff, decide_eq_true_eq, not_le,
+        zero_lt_one]
+    case inr h_pos =>
+      rw [le_sup_iff]
+      left
+      simp only [fslIverson, Int.reduceNeg, fslMul]
+      rw [unitInterval.iteOneZero_le]
+      intro h
+      simp only [is_in_ico, Int.reduceNeg, slExists_apply, slEquals, const, var, Subtype.exists,
+        Set.mem_Ico, exists_prop] at h
+      obtain ⟨i, ⟨h_l, h_u⟩, h_eq⟩ := h
+      have h_0 : 0 ≤ i := by {
+          apply lt_of_le_of_ne h_l
+          qify
+          rw [h_eq]
+          exact h_pos.symm
+      }
+      rw [unitInterval.iteOneZero_pos, unitInterval.iteOneZero_pos]
+      · simp only [mul_one, le_refl]
+      · simp only [is_in_ico, slExists_apply, slEquals, const, var, Subtype.exists, Set.mem_Ico,
+          exists_prop]
+        use i, ⟨h_0, h_u⟩
+      · simp only [slExp, leq, const, var, decide_eq_true_eq]
+        rw [← h_eq]
+        qify at h_0
+        exact h_0
+  · apply safeTuple_seq _ (producer_sound₁ y)
+    exact safeTuple_seq _ (producer_sound₂ y) (producer_sound₃ y)
+
 
 theorem channel_sound (y : ℕ) (p : unitInterval) :
     ⊢ [[rInv y]]
-    ⦃(⁅<leq (const 0) (var "y2")>⁆ ⊓ ⁅<lt (var "y2") (const ↑y)>⁆)
-        ⬝ <exp (constP p) (inc (var "y2"))>
-      ⊔ ~⁅<leq (const 0) (var "y2")>⁆ ⦄
+    ⦃⁅is_in_ico "y2" 0 y⁆ ⬝ <exp (constP p) (var "y2")>
+      ⊔ ~⁅<leq (const 0) (var "y2")>⁆ ⊓ ⁅is_in_ico "y2" (-1) y⁆ ⦄
     channel p
     ⦃ fTrue ⦄ := sorry
 
 theorem consumer_sound (y : ℕ) :
     ⊢ [[rInv y]]
-    ⦃⁅<leq (const 0) (var "y3")>⁆ ⊓ ⁅<lt (var "y3") (const ↑y)>⁆
-        ⊓ (var "l" === sub (const ↑y) (inc (var "y3")))
-      ⊔ ~⁅<leq (const 0) (var "y3")>⁆ ⊓ var "l" === const ↑y ⦄
+    ⦃⁅is_in_ico "y3" (-1) y⁆ ⊓ var "l" === sub (dec $ const y) (var "y3")⦄
   consumer
   ⦃ var "l" === const ↑y ⦄ := sorry
 
 theorem producerConsumer_sound (y : ℕ) (p : unitInterval) :
     ⊢ emp
-    ⦃<exp (constP p) (const y)> ⋆ [[rInv y]]⦄
+    ⦃<exp (constP p) (dec $ const y)> ⋆ [[rInv y]]⦄
     producerConsumer y p
     ⦃var "l" === const y ⋆ [[rInv y]]⦄ := by
   unfold producerConsumer
